code/experimental/P256/Hacl.Impl.ECDSA.P256SHA256.Verification.fst
@@ -13,11 +13,11 @@ open Hacl.Impl.P256
 open Hacl.Spec.P256.MontgomeryMultiplication
 open Hacl.Impl.ECDSA.MontgomeryMultiplication
 open Hacl.Impl.ECDSA.MM.Exponent
+open Hacl.Spec.P256.Ladder
 
 open Hacl.Spec.ECDSAP256.Definition
 open Hacl.Spec.ECDSA
 open Hacl.Spec.P256 
-open Hacl.Spec.P256.Ladder
 open Hacl.Spec.P256.Lemmas
 
 open Hacl.Impl.P256.PointAdd
